sandbox/ComprehensionNotation.v
@@ -1,1 +1,29 @@
-../src/ComprehensionNotation.v
+(** We combine replacement with comprehension as [(m for x : s if p)],
+    which is more flexible than comprehension alone [{x : s & p}].
+    This will be especially useful for constructing [Join]s.  *)
+
+Notation "( m 'for' x1 : t1 )" :=
+  (fun x1 : t1 => m)
+  (at level 0, x1 at level 99) : type_scope.
+Notation "( m 'for' x1 : t1 'if' t2 )" :=
+  (fun x : {x1 : t1 & t2} => match x with existT x1 _ => m end)
+  (at level 0, x1 at level 99) : type_scope.
+Notation "( m 'for' x1 : t1 'if' t2 'if' t3 )" :=
+  (fun x : {x1 : t1 & t2 & t3} => match x with existT2 x1 _ _ => m end)
+  (at level 0, x1 at level 99) : type_scope.
+Notation "( m 'for' x1 : t1 'for' x2 : t2 )" :=
+  (fun x : t1 * t2 => match x with (x1, x2) => m end)
+  (at level 0, x1 at level 99, x2 at level 99) : type_scope.
+Notation "( m 'for' x1 : t1 'for' x2 : t2 'if' t3 )" :=
+  (fun x : sigT (fun x12 : t1 * t2 => let (x1, x2) := x12 in t3) =>
+  match x with existT (x1, x2) _ => m end)
+  (at level 0, x1 at level 99, x2 at level 99) : type_scope.
+Notation "( m 'for' x1 : t1 'for' x2 : t2 'if' t3 )" :=
+  (fun x : sigT (fun x12 : t1 * t2 => let (x1, x2) := x12 in t3) =>
+  match x with existT (x1, x2) _ => m end)
+  (at level 0, x1 at level 99, x2 at level 99) : type_scope.
+Notation "( m 'for' x1 : t1 'for' x2 : t2 'if' t3 'if' t4 )" :=
+  (fun x : sigT2 (fun x12 : t1 * t2 => let (x1, x2) := x12 in t3)
+                 (fun x12 : t1 * t2 => let (x1, x2) := x12 in t4) =>
+  match x with existT2 (x1, x2) _ _ => m end)
+  (at level 0, x1 at level 99, x2 at level 99) : type_scope.
